James C - finished chapter 09

isabelle/Chapter09_2_Typechecking.thy
@@ -4,29 +4,18 @@ begin
 
 inductive typecheck :: "type env => expr => type => bool"
 where tc_var [simp]: "lookup gam x = Some t ==> typecheck gam (Var x) t"
-    | tc_str [simp]: "typecheck gam (Str s) StrType"
-    | tc_num [simp]: "typecheck gam (Num n) NumType"
-    | tc_plus [simp]: "typecheck gam e1 NumType ==> typecheck gam e2 NumType ==> 
-                    typecheck gam (Plus e1 e2) NumType"
-    | tc_times [simp]: "typecheck gam e1 NumType ==> typecheck gam e2 NumType ==> 
-                    typecheck gam (Times e1 e2) NumType"
-    | tc_cat [simp]: "typecheck gam e1 StrType ==> typecheck gam e2 StrType ==>
-                    typecheck gam (Cat e1 e2) StrType"
-    | tc_len [simp]: "typecheck gam e StrType ==> typecheck gam (Len e) NumType"
-    | tc_let [simp]: "typecheck gam e1 t1 ==> typecheck (extend gam t1) e2 t2 ==> 
-                    typecheck gam (Let e1 e2) t2"
+    | tc_zero [simp]: "typecheck gam Zero Nat"
+    | tc_suc [simp]: "typecheck gam e Nat ==> typecheck gam (Suc e) Nat"
+    | tc_rec [simp]: "typecheck gam et Nat ==> typecheck gam e0 t ==> 
+                typecheck (extend (extend gam t) Nat) es t ==> typecheck gam (Rec et e0 es) t"
     | tc_lam [simp]: "typecheck (extend gam t1) e t2 ==> typecheck gam (Lam t1 e) (Arrow t1 t2)"
     | tc_appl [simp]: "typecheck gam e1 (Arrow t2 t) ==> typecheck gam e2 t2 ==> 
-                    typecheck gam (Appl e1 e2) t"
+                typecheck gam (Appl e1 e2) t"
 
 inductive_cases [elim!]: "typecheck gam (Var x) t"
-inductive_cases [elim!]: "typecheck gam (Str s) t"
-inductive_cases [elim!]: "typecheck gam (Num n) t"
-inductive_cases [elim!]: "typecheck gam (Plus e1 e2) t"
-inductive_cases [elim!]: "typecheck gam (Times e1 e2) t"
-inductive_cases [elim!]: "typecheck gam (Cat e1 e2) t"
-inductive_cases [elim!]: "typecheck gam (Len e) t"
-inductive_cases [elim!]: "typecheck gam (Let e1 e2) t"
+inductive_cases [elim!]: "typecheck gam Zero t"
+inductive_cases [elim!]: "typecheck gam (Suc e) t"
+inductive_cases [elim!]: "typecheck gam (Rec et e0 es) t"
 inductive_cases [elim!]: "typecheck gam (Lam t1 e) t"
 inductive_cases [elim!]: "typecheck gam (Appl e1 e2) t"
 
