isabelle/Chapter09_3_Evaluation.thy
@@ -4,68 +4,65 @@ begin
 
 primrec is_val :: "expr => bool"
 where "is_val (Var v) = False"
-    | "is_val (Num x) = True"
-    | "is_val (Str s) = True"
-    | "is_val (Plus e1 e2) = False"
-    | "is_val (Times e1 e2) = False"
-    | "is_val (Cat e1 e2) = False"
-    | "is_val (Len e) = False"
-    | "is_val (Let e1 e2) = False"
+    | "is_val Zero = True"
+    | "is_val (Suc e) = is_val e"
+    | "is_val (Rec et e0 es) = False"
     | "is_val (Lam t e) = True"
     | "is_val (Appl e1 e2) = False"
 
 inductive eval :: "expr => expr => bool"
-where eval_plus_1 [simp]: "eval (Plus (Num n1) (Num n2)) (Num (n1 + n2))"
-    | eval_plus_2 [simp]: "eval e1 e1' ==> eval (Plus e1 e2) (Plus e1' e2)"
-    | eval_plus_3 [simp]: "is_val e1 ==> eval e2 e2' ==> eval (Plus e1 e2) (Plus e1 e2')"
-    | eval_times_1 [simp]: "eval (Times (Num n1) (Num n2)) (Num (n1 * n2))"
-    | eval_times_2 [simp]: "eval e1 e1' ==> eval (Times e1 e2) (Times e1' e2)"
-    | eval_times_3 [simp]: "is_val e1 ==> eval e2 e2' ==> eval (Times e1 e2) (Times e1 e2')"
-    | eval_cat_1 [simp]: "eval (Cat (Str n1) (Str n2)) (Str (n1 @ n2))"
-    | eval_cat_2 [simp]: "eval e1 e1' ==> eval (Cat e1 e2) (Cat e1' e2)"
-    | eval_cat_3 [simp]: "is_val e1 ==> eval e2 e2' ==> eval (Cat e1 e2) (Cat e1 e2')"
-    | eval_len_1 [simp]: "eval (Len (Str n1)) (Num (int (length n1)))"
-    | eval_len_2 [simp]: "eval e1 e1' ==> eval (Len e1) (Len e1')"
-    | eval_let_1 [simp]: "is_val e1 ==> eval (Let e1 e2) (subst e1 e2)"
-    | eval_let_2 [simp]: "eval e1 e1' ==> eval (Let e1 e2) (Let e1' e2)"
+where eval_suc [simp]: "eval e e' ==> eval (Suc e) (Suc e')"
+    | eval_rec_1 [simp]: "eval et et' ==> eval (Rec et e0 es) (Rec et e0 es)"
+    | eval_rec_2 [simp]: "eval (Rec Zero e0 es) e0"
+    | eval_rec_3 [simp]: "is_val et ==> 
+            eval (Rec (Suc et) e0 es) (subst (Rec et e0 es) (subst et es))"
     | eval_appl_1 [simp]: "eval e1 e1' ==> eval (Appl e1 e2) (Appl e1' e2)"
     | eval_appl_2 [simp]: "is_val e1 ==> eval e2 e2' ==> eval (Appl e1 e2) (Appl e1 e2')"
     | eval_appl_3 [simp]: "is_val e2 ==> eval (Appl (Lam t2 e1) e2) (subst e2 e1)"
 
-lemma canonical_num: "is_val e ==> typecheck gam e NumType ==> EX n. e = Num n"
+lemma canonical_nat: "is_val e ==> typecheck gam e Nat ==> 
+          e = Zero | (EX e'. e = Suc e' & typecheck gam e' Nat)"
 by (induction e, auto)
 
-lemma canonical_str: "is_val e ==> typecheck gam e StrType ==> EX n. e = Str n"
-by (induction e, auto)
+lemma canonical_nat_no_vars: "is_val e ==> typecheck gam e Nat ==> typecheck gam' e Nat"
+by (induction e, auto) 
 
 lemma canonical_arrow: "is_val e ==> typecheck gam e (Arrow t1 t2) ==> 
               EX e'. e = Lam t1 e' & typecheck (extend gam t1) e' t2"
 by (induction e, auto)
 
 theorem preservation: "eval e e' ==> typecheck gam e t ==> typecheck gam e' t"
-by (induction e e' arbitrary: t rule: eval.induct, fastforce+)
+proof (induction e e' arbitrary: t rule: eval.induct)
+case eval_suc 
+  thus ?case by fastforce
+next case eval_rec_1 
+  thus ?case by fastforce
+next case eval_rec_2 
+  thus ?case by fastforce
+next case (eval_rec_3 et e0 es)
+  from eval_rec_3 canonical_nat_no_vars have "typecheck (extend gam t) (subst et es) t" by auto
+  with eval_rec_3 show ?case by fastforce
+next case eval_appl_1 
+  thus ?case by fastforce
+next case eval_appl_2 
+  thus ?case by fastforce
+next case eval_appl_3 
+  thus ?case by fastforce
+qed
 
 theorem progress: "typecheck gam e t ==> gam = empty_env ==> is_val e | (EX e'. eval e e')"
 proof (induction gam e t rule: typecheck.induct)
 case tc_var
   thus ?case by simp
-next case tc_str
+next case tc_zero
   thus ?case by simp
-next case tc_num
+next case tc_suc
+  thus ?case by (metis eval_suc is_val.simps(3))
+next case tc_rec
+  thus ?case by (metis eval_rec_1 eval_rec_2 eval_rec_3 is_val.simps(3) canonical_nat)
+next case tc_lam
   thus ?case by simp
-next case (tc_plus gam e1 e2)
-  thus ?case by (metis eval_plus_1 eval_plus_2 eval_plus_3 canonical_num)
-next case (tc_times gam e1 e2)
-  thus ?case by (metis eval_times_1 eval_times_2 eval_times_3 canonical_num)
-next case (tc_cat gam e1 e2)
-  thus ?case by (metis eval_cat_1 eval_cat_2 eval_cat_3 canonical_str)
-next case (tc_len gam e)
-  thus ?case by (metis eval_len_1 eval_len_2 canonical_str)
-next case (tc_let gam e1 t1 e2 t2)
-  thus ?case by (metis eval_let_1 eval_let_2)
-next case (tc_lam gam t1 e t2)
-  thus ?case by simp
-next case (tc_appl gam e1 t2 t e2)
+next case tc_appl
   thus ?case by (metis eval_appl_1 eval_appl_2 eval_appl_3 canonical_arrow)
 qed
 
