isabelle/Chapter09_1_Language.thy
@@ -3,55 +3,40 @@ imports DeBruijnEnvironment
 begin
 
 datatype type = 
-  NumType 
-| StrType
+  Nat
 | Arrow type type
 
 datatype expr = 
   Var var
-| Num int
-| Str string
-| Plus expr expr
-| Times expr expr
-| Cat expr expr
-| Len expr
-| Let expr expr
+| Zero
+| Suc expr
+| Rec expr expr expr
 | Lam type expr
 | Appl expr expr
 
 primrec insert :: "var => expr => expr"
 where "insert n (Var v) = Var (incr n v)"
-    | "insert n (Num x) = Num x"
-    | "insert n (Str s) = Str s"
-    | "insert n (Plus e1 e2) = Plus (insert n e1) (insert n e2)"
-    | "insert n (Times e1 e2) = Times (insert n e1) (insert n e2)"
-    | "insert n (Cat e1 e2) = Cat (insert n e1) (insert n e2)"
-    | "insert n (Len e) = Len (insert n e)"
-    | "insert n (Let e1 e2) = Let (insert n e1) (insert (next n) e2)"
+    | "insert n Zero = Zero"
+    | "insert n (Suc e) = Suc (insert n e)"
+    | "insert n (Rec et e0 es) = Rec (insert n et) (insert n e0) (insert (next (next n)) es)"
     | "insert n (Lam t e) = Lam t (insert (next n) e)"
     | "insert n (Appl e1 e2) = Appl (insert n e1) (insert n e2)"
 
 primrec remove :: "var => expr => expr"
 where "remove n (Var v) = Var (subr n v)"
-    | "remove n (Num x) = Num x"
-    | "remove n (Str s) = Str s"
-    | "remove n (Plus e1 e2) = Plus (remove n e1) (remove n e2)"
-    | "remove n (Times e1 e2) = Times (remove n e1) (remove n e2)"
-    | "remove n (Cat e1 e2) = Cat (remove n e1) (remove n e2)"
-    | "remove n (Len e) = Len (remove n e)"
-    | "remove n (Let e1 e2) = Let (remove n e1) (remove (next n) e2)"
+    | "remove n Zero = Zero"
+    | "remove n (Suc e) = Suc (remove n e)"
+    | "remove n (Rec et e0 es) = Rec (remove n et) (remove n e0) (remove (next (next n)) es)"
     | "remove n (Lam t e) = Lam t (remove (next n) e)"
     | "remove n (Appl e1 e2) = Appl (remove n e1) (remove n e2)"
 
 primrec subst' :: "var => expr => expr => expr"
 where "subst' n e' (Var v) = (if v = n then e' else Var v)"
-    | "subst' n e' (Num x) = Num x"
-    | "subst' n e' (Str s) = Str s"
-    | "subst' n e' (Plus e1 e2) = Plus (subst' n e' e1) (subst' n e' e2)"
-    | "subst' n e' (Times e1 e2) = Times (subst' n e' e1) (subst' n e' e2)"
-    | "subst' n e' (Cat e1 e2) = Cat (subst' n e' e1) (subst' n e' e2)"
-    | "subst' n e' (Len e) = Len (subst' n e' e)"
-    | "subst' n e' (Let e1 e2) = Let (subst' n e' e1) (subst' (next n) (insert first e') e2)"
+    | "subst' n e' Zero = Zero"
+    | "subst' n e' (Suc e) = Suc (subst' n e' e)"
+    | "subst' n e' (Rec et e0 es) = 
+                      Rec (subst' n e' et) (subst' n e' e0) 
+                          (subst' (next (next n)) (insert first (insert first e')) es)"
     | "subst' n e' (Lam t e) = Lam t (subst' (next n) (insert first e') e)"
     | "subst' n e' (Appl e1 e2) = Appl (subst' n e' e1) (subst' n e' e2)"
 
